Replace module types with type classes
Also move the explicit definition of the State record type (and
corresponding instances of Independent) to a separate file. Finally,
insert "using" to reduce warnings.

assembly/Machine.v
@@ -6,349 +6,255 @@ Require Import Assembly.Dec.
 Require Import Assembly.Operations.
 Require Assembly.OpCodes.
 
-From RecordUpdate Require Import RecordSet.
 
 (* Global parameters! *)
 Context
-  (memStart: nat) (* TODO: Use B64 instead? *)
-  (memSize: nat)
-  (inputImages : list (Image B8)).
+  (available': B64 -> bool)
+  (allInputImages' : list (Image B8)).
 
-Module CT <: core_type'.
+Instance concreteParams0 : MachineParams0 :=
+{
+  Addr := B64;
+  H_eqdec := (ltac:(typeclasses eauto) : EqDec B64);
+  available := available';
+  offset := fun (z: Z) (a: B64) => toB64 (z + a);
+  Cell := B8;
 
-  Definition Addr := B64.
-  Definition H_eqdec := (ltac:(typeclasses eauto) : EqDec B64).
-  Definition available := fun (a: B64) => as_bool (decision (memStart <= a /\ a < memStart + memSize)).
-  Definition offset := fun (z: Z) (a: B64) => toB64 (z + a).
-  Definition Cell := B8.
+  InputColor := B8;
+  allInputImages := allInputImages';
 
-  Definition InputColor := B8.
-  Definition allInputImages := inputImages.
+  OutputColor := B64 * B64 * B64;
+  Char := B32;
+  Byte := B8;
+  Sample := B16;
+}.
 
-  Definition OutputColor : Type := B64 * B64 * B64.
-  Definition Char := B32.
-  Definition Byte := B8.
-  Definition Sample := B16.
+Section machine_section.
 
-  Include machine_type_defs.
+  (** We leave these assumptions abstract in order improve proof search.
+      In Concete.v we have shown that they hold in our standard model. *)
 
-  Record actual_State :=
-  mkState {
-    state_memory: Memory;
-    state_pc: Addr;
-    state_sp: Addr;
-    state_inp: Image InputColor;
-    state_image: Image (option OutputColor);
-    state_bytes: list Byte;
-    state_chars: list Char;
-    state_sound: Sound;
-    state_log: list OutputFrame;
-  }.
-  Instance etaState : Settable _ :=
-    settable! mkState <state_memory;
-                       state_pc;
-                       state_sp;
-                       state_inp;
-                       state_image;
-                       state_bytes;
-                       state_chars;
-                       state_sound;
-                       state_log>.
-  Definition State := actual_State.
-  Definition M := EST State.
-  Definition H_mon := est_smonad State.
+  Context {MP1: @MachineParams1 concreteParams0}.
+  Context {MP2: @MachineParams2 concreteParams0 MP1}.
 
-  Local Ltac crush :=
-    let s := fresh in try split; intro s; intros; destruct s; reflexivity.
+  Existing Instance H_mon.
 
-  Local Ltac derive_proj f :=
-    refine {|
-        proj := f;
-        update s m := set f (fun _ => m) s;
-    |}; crush.
+  Definition nextN (n: nat) : M nat :=
+    let* bytes := next n in
+    ret (fromLittleEndian bytes).
 
-  Definition MEM : Proj State Memory. derive_proj state_memory. Defined.
-  Definition PC : Proj State Addr. derive_proj state_pc. Defined.
-  Definition SP : Proj State Addr. derive_proj state_sp. Defined.
-  Definition INP : Proj State (Image InputColor). derive_proj state_inp. Defined.
-  Definition OUT_CHARS : Proj State (list Char). derive_proj state_chars. Defined.
-  Definition OUT_BYTES : Proj State (list Byte). derive_proj state_bytes. Defined.
-  Definition OUT_SOUND : Proj State Sound. derive_proj state_sound. Defined.
-  Definition OUT_IMAGE : Proj State (Image (option OutputColor)). derive_proj state_image. Defined.
-  Definition LOG : Proj State (list OutputFrame). derive_proj state_log. Defined.
+  Definition push64 (z: Z) : M unit :=
+    pushMany (toLittleEndian 8 z).
 
-  Instance independent_MEM_IMAGE: Independent MEM OUT_IMAGE. crush. Defined.
-  Instance independent_MEM_BYTES: Independent MEM OUT_BYTES. crush. Defined.
-  Instance independent_MEM_CHARS: Independent MEM OUT_CHARS. crush. Defined.
-  Instance independent_MEM_SOUND: Independent MEM OUT_SOUND. crush. Defined.
-  Instance independent_MEM_LOG:   Independent MEM LOG. crush. Defined.
-  Instance independent_MEM_INP:   Independent MEM INP. crush. Defined.
-  Instance independent_MEM_PC:    Independent MEM PC. crush. Defined.
-  Instance independent_MEM_SP:    Independent MEM SP. crush. Defined.
+  Definition popN : M nat :=
+    let* bytes := popMany 8 in
+    ret (fromLittleEndian bytes).
 
-  Instance independent_IMAGE_BYTES: Independent OUT_IMAGE OUT_BYTES. crush. Defined.
-  Instance independent_IMAGE_CHARS: Independent OUT_IMAGE OUT_CHARS. crush. Defined.
-  Instance independent_IMAGE_SOUND: Independent OUT_IMAGE OUT_SOUND. crush. Defined.
-  Instance independent_IMAGE_LOG:   Independent OUT_IMAGE LOG. crush. Defined.
-  Instance independent_IMAGE_INP:   Independent OUT_IMAGE INP. crush. Defined.
-  Instance independent_IMAGE_PC:    Independent OUT_IMAGE PC. crush. Defined.
-  Instance independent_IMAGE_SP:    Independent OUT_IMAGE SP. crush. Defined.
+  Definition pop64 : M B64 :=
+    let* x := popN in
+    ret (toB64 x).
 
-  Instance independent_BYTES_CHARS: Independent OUT_BYTES OUT_CHARS. crush. Defined.
-  Instance independent_BYTES_SOUND: Independent OUT_BYTES OUT_SOUND. crush. Defined.
-  Instance independent_BYTES_LOG:   Independent OUT_BYTES LOG. crush. Defined.
-  Instance independent_BYTES_INP:   Independent OUT_BYTES INP. crush. Defined.
-  Instance independent_BYTES_PC:    Independent OUT_BYTES PC. crush. Defined.
-  Instance independent_BYTES_SP:    Independent OUT_BYTES SP. crush. Defined.
+  Definition loadN (n: nat) (a: Z) : M nat :=
+    let* bytes := loadMany n (toB64 a) in
+    ret (fromLittleEndian bytes).
 
-  Instance independent_CHARS_SOUND: Independent OUT_CHARS OUT_SOUND. crush. Defined.
-  Instance independent_CHARS_LOG:   Independent OUT_CHARS LOG. crush. Defined.
-  Instance independent_CHARS_INP:   Independent OUT_CHARS INP. crush. Defined.
-  Instance independent_CHARS_PC:    Independent OUT_CHARS PC. crush. Defined.
-  Instance independent_CHARS_SP:    Independent OUT_CHARS SP. crush. Defined.
+  Definition storeZ (n: nat) (a: Z) (x: Z) : M unit :=
+    storeMany (toB64 a) (map Some (toLittleEndian n x)).
 
-  Instance independent_SOUND_LOG: Independent OUT_SOUND LOG. crush. Defined.
-  Instance independent_SOUND_INP: Independent OUT_SOUND INP. crush. Defined.
-  Instance independent_SOUND_PC:  Independent OUT_SOUND PC. crush. Defined.
-  Instance independent_SOUND_SP:  Independent OUT_SOUND SP. crush. Defined.
+  Import OpCodes.
 
-  Instance independent_LOG_INP: Independent LOG INP. crush. Defined.
-  Instance independent_LOG_PC:  Independent LOG PC. crush. Defined.
-  Instance independent_LOG_SP:  Independent LOG SP. crush. Defined.
+  (* Without [noind] solving obligations seems to go on forever.
+     Alas, this still generated 257 equations... *)
+  Equations(noind) oneStep' (op: nat) : M unit :=
+    oneStep' NOP := ret tt;
 
-  Instance independent_INP_PC: Independent INP PC. crush. Defined.
-  Instance independent_INP_SP: Independent INP SP. crush. Defined.
-
-  Instance independent_PC_SP: Independent PC SP. crush. Defined.
-End CT.
-
-Export CT.
-
-Module CM := core_module CT.
-Export CM.
-
-Identity Coercion id_Addr : Addr >-> B64.
-Identity Coercion id_Cell : Cell >-> B8.
-Identity Coercion id_InputColor : InputColor >-> B8.
-Identity Coercion id_Char : Char >-> B32.
-Identity Coercion id_Byte : Byte >-> B8.
-Identity Coercion id_Sample : Sample >-> B16.
-
-
-Definition nextN (n: nat) : M nat :=
-  let* bytes := next n in
-  ret (fromLittleEndian bytes).
-
-Definition push64 (z: Z) : M unit :=
-  pushMany (toLittleEndian 8 z).
-
-Definition popN : M nat :=
-  let* bytes := popMany 8 in
-  ret (fromLittleEndian bytes).
-
-Definition pop64 : M B64 :=
-  let* x := popN in
-  ret (toB64 x).
-
-Definition loadN (n: nat) (a: Z) : M nat :=
-  let* bytes := loadMany n (toB64 a) in
-  ret (fromLittleEndian bytes).
-
-Definition storeZ (n: nat) (a: Z) (x: Z) : M unit :=
-  storeMany (toB64 a) (map Some (toLittleEndian n x)).
-
-Import OpCodes.
-
-(* Without [noind] solving obligations seems to go on forever.
-   Alas, this still generated 257 equations... *)
-Equations(noind) oneStep' (op: nat) : M unit :=
-  oneStep' NOP := ret tt;
-
-  oneStep' JUMP :=
-    let* a := popN in
-    put' PC (toB64 a);
-
-  oneStep' JUMP_ZERO :=
-      let* o := nextN 1 in
-      let* x := popN in
-      (if (decision (x = 0))
-       then
-         let* pc := get' PC in
-         put' PC (offset (signed (toB8 o)) pc)
-       else
-         ret tt);
-
-  oneStep' SET_SP :=
-      let* a := pop64 in
-      put' SP a;
-
-  oneStep' GET_PC =>
-      let* a := get' PC in
-      push64 a;
-
-  oneStep' GET_SP :=
-      let* a := get' SP in
-      push64 a;
-
-  oneStep' PUSH0 :=
-      push64 0;
-
-  oneStep' PUSH1 :=
-      let* x := nextN 1 in
-      push64 x;
-
-  oneStep' PUSH2 :=
-      let* x := nextN 2 in
-      push64 x;
-
-  oneStep' PUSH4 :=
-      let* x := nextN 4 in
-      push64 x;
-
-  oneStep' PUSH8 :=
-      let* x := nextN 8 in
-      push64 x;
-
-  oneStep' SIGX1 :=
-      let* x := popN in
-      push64 (signed (toB8 x));
-
-  oneStep' SIGX2 :=
-      let* x := popN in
-      push64 (signed (toB16 x));
-
-  oneStep' SIGX4 :=
-      let* x := popN in
-      push64 (signed (toB32 x));
-
-  oneStep' LOAD1 :=
+    oneStep' JUMP :=
       let* a := popN in
-      let* x := loadN 1 a in
-      push64 x;
+      put' PC (toB64 a);
 
-  oneStep' LOAD2 :=
-      let* a := popN in
-      let* x := loadN 2 a in
-      push64 x;
+    oneStep' JUMP_ZERO :=
+        let* o := nextN 1 in
+        let* x := popN in
+        (if (decision (x = 0))
+         then
+           let* pc := get' PC in
+           put' PC (offset (signed (toB8 o)) pc)
+         else
+           ret tt);
 
-  oneStep' LOAD4 :=
-      let* a := popN in
-      let* x := loadN 4 a in
-      push64 x;
+    oneStep' SET_SP :=
+        let* a := pop64 in
+        put' SP a;
 
-  oneStep' LOAD8 :=
-      let* a := popN in
-      let* x := loadN 8 a in
-      push64 x;
+    oneStep' GET_PC =>
+        let* a := get' PC in
+        push64 (a: B64);
 
-  oneStep' STORE1 :=
-      let* a := popN in
-      let* x := popN in
-      storeZ 1 a x;
+    oneStep' GET_SP :=
+        let* a := get' SP in
+        push64 (a: B64);
 
-  oneStep' STORE2 :=
-      let* a := popN in
-      let* x := popN in
-      storeZ 2 a x;
+    oneStep' PUSH0 :=
+        push64 0;
 
-  oneStep' STORE4 :=
-      let* a := popN in
-      let* x := popN in
-      storeZ 4 a x;
+    oneStep' PUSH1 :=
+        let* x := nextN 1 in
+        push64 x;
 
-  oneStep' STORE8 :=
-      let* a := popN in
-      let* x := popN in
-      storeZ 8 a x;
+    oneStep' PUSH2 :=
+        let* x := nextN 2 in
+        push64 x;
 
-  oneStep' ADD :=
-      let* x := popN in
-      let* y := popN in
-      push64 (x + (y:nat));
+    oneStep' PUSH4 :=
+        let* x := nextN 4 in
+        push64 x;
 
-  oneStep' MULT :=
-      let* x := popN in
-      let* y := popN in
-      push64 (x * (y:nat));
+    oneStep' PUSH8 :=
+        let* x := nextN 8 in
+        push64 x;
 
-  oneStep' DIV :=
-      let* x := popN in
-      let* y := popN in
-      push64 (if decision (x=0) then 0 else (y:nat) / x);
+    oneStep' SIGX1 :=
+        let* x := popN in
+        push64 (signed (toB8 x));
 
-  oneStep' REM :=
-      let* x := popN in
-      let* y := popN in
-      push64 (if decision (x=0) then 0 else (y:nat) mod x);
+    oneStep' SIGX2 :=
+        let* x := popN in
+        push64 (signed (toB16 x));
 
-  oneStep' LT :=
-      let* x := popN in
-      let* y := popN in
-      push64 (if decision (y < x) then -1 else 0);
+    oneStep' SIGX4 :=
+        let* x := popN in
+        push64 (signed (toB32 x));
 
-  oneStep' AND :=
-      let* x := pop64 in
-      let* y := pop64 in
-      push64 (Vector.map2 andb x y : B64);
+    oneStep' LOAD1 :=
+        let* a := popN in
+        let* x := loadN 1 a in
+        push64 x;
 
-  oneStep' OR :=
-      let* x := pop64 in
-      let* y := pop64 in
-      push64 (Vector.map2 orb x y : B64);
+    oneStep' LOAD2 :=
+        let* a := popN in
+        let* x := loadN 2 a in
+        push64 x;
 
-  oneStep' NOT :=
-      let* x := pop64 in
-      push64 (Vector.map negb x : B64);
+    oneStep' LOAD4 :=
+        let* a := popN in
+        let* x := loadN 4 a in
+        push64 x;
 
-  oneStep' XOR :=
-      let* x := pop64 in
-      let* y := pop64 in
-      push64 (Vector.map2 xorb x y : B64);
+    oneStep' LOAD8 :=
+        let* a := popN in
+        let* x := loadN 8 a in
+        push64 x;
 
-  oneStep' READ_FRAME :=
-      let* i := popN in
-      let* pair := readFrame (i: nat) in
-      push64 (fst pair);;
-      push64 (snd pair);
+    oneStep' STORE1 :=
+        let* a := popN in
+        let* x := popN in
+        storeZ 1 a x;
 
-  oneStep' READ_PIXEL :=
-      let* y := popN in
-      let* x := popN in
-      let* c := readPixel x y in
-      push64 c;
+    oneStep' STORE2 :=
+        let* a := popN in
+        let* x := popN in
+        storeZ 2 a x;
 
-  oneStep' NEW_FRAME :=
-      let* r := popN in
-      let* h := popN in
-      let* w := popN in
-      newFrame w h r;
+    oneStep' STORE4 :=
+        let* a := popN in
+        let* x := popN in
+        storeZ 4 a x;
 
-  oneStep' SET_PIXEL :=
-      let* b := pop64 in
-      let* g := pop64 in
-      let* r := pop64 in
-      let* y := popN in
-      let* x := popN in
-      setPixel x y (r, g, b);
+    oneStep' STORE8 :=
+        let* a := popN in
+        let* x := popN in
+        storeZ 8 a x;
 
-  oneStep' ADD_SAMPLE :=
-      let* r := popN in
-      let* l := popN in
-      addSample (toB16 l) (toB16 r);
+    oneStep' ADD :=
+        let* x := popN in
+        let* y := popN in
+        push64 (x + (y:nat));
 
-  oneStep' PUT_CHAR :=
-      let* c := popN in
-      putChar (toB32 c);
+    oneStep' MULT :=
+        let* x := popN in
+        let* y := popN in
+        push64 (x * (y:nat));
 
-  oneStep' PUT_BYTE :=
-      let* b := popN in
-      putByte (toB8 b);
+    oneStep' DIV :=
+        let* x := popN in
+        let* y := popN in
+        push64 (if decision (x=0) then 0 else (y:nat) / x);
 
-  oneStep' _ := err.
+    oneStep' REM :=
+        let* x := popN in
+        let* y := popN in
+        push64 (if decision (x=0) then 0 else (y:nat) mod x);
 
-Definition oneStep : M bool :=
-  let* op := nextN 1 in
-  match op with
-  | EXIT => ret false
-  | _ => oneStep' op;; ret true
-  end.
+    oneStep' LT :=
+        let* x := popN in
+        let* y := popN in
+        push64 (if decision (y < x) then -1 else 0);
+
+    oneStep' AND :=
+        let* x := pop64 in
+        let* y := pop64 in
+        push64 (Vector.map2 andb x y : B64);
+
+    oneStep' OR :=
+        let* x := pop64 in
+        let* y := pop64 in
+        push64 (Vector.map2 orb x y : B64);
+
+    oneStep' NOT :=
+        let* x := pop64 in
+        push64 (Vector.map negb x : B64);
+
+    oneStep' XOR :=
+        let* x := pop64 in
+        let* y := pop64 in
+        push64 (Vector.map2 xorb x y : B64);
+
+    oneStep' READ_FRAME :=
+        let* i := popN in
+        let* pair := readFrame (i: nat) in
+        push64 (fst pair);;
+        push64 (snd pair);
+
+    oneStep' READ_PIXEL :=
+        let* y := popN in
+        let* x := popN in
+        let* c := readPixel x y in
+        push64 (c: B8);
+
+    oneStep' NEW_FRAME :=
+        let* r := popN in
+        let* h := popN in
+        let* w := popN in
+        newFrame w h r;
+
+    oneStep' SET_PIXEL :=
+        let* b := pop64 in
+        let* g := pop64 in
+        let* r := pop64 in
+        let* y := popN in
+        let* x := popN in
+        setPixel x y (r, g, b);
+
+    oneStep' ADD_SAMPLE :=
+        let* r := popN in
+        let* l := popN in
+        addSample (toB16 l) (toB16 r);
+
+    oneStep' PUT_CHAR :=
+        let* c := popN in
+        putChar (toB32 c);
+
+    oneStep' PUT_BYTE :=
+        let* b := popN in
+        putByte (toB8 b);
+
+    oneStep' _ := err.
+
+  Definition oneStep : M bool :=
+    let* op := nextN 1 in
+    match op with
+    | EXIT => ret false
+    | _ => oneStep' op;; ret true
+    end.
+
+End machine_section.
