assembly/Concrete.v
@@ -1,0 +1,167 @@
+Require Import Equations.Equations.
+
+Require Import Assembly.Mon.
+Require Import Assembly.Bits.
+Require Import Assembly.Dec.
+Require Import Assembly.Operations.
+Require Import Assembly.Machine.
+
+From RecordUpdate Require Import RecordSet.
+
+(** The purpose of this file is to prove the (rather trivial) fact that
+the initial error state monad over the obvious record type does indeed
+satisfy the constraints in [MachineParams1].*)
+
+Record State :=
+mkState {
+  state_memory: Memory;
+  state_pc: Addr;
+  state_sp: Addr;
+  state_inp: Image InputColor;
+  state_image: Image (option OutputColor);
+  state_bytes: list Byte;
+  state_chars: list Char;
+  state_sound: Sound;
+  state_log: list OutputFrame;
+}.
+Instance etaState : Settable _ :=
+  settable! mkState <state_memory;
+                     state_pc;
+                     state_sp;
+                     state_inp;
+                     state_image;
+                     state_bytes;
+                     state_chars;
+                     state_sound;
+                     state_log>.
+
+Local Ltac crush :=
+  let s := fresh in try split; intro s; intros; destruct s; reflexivity.
+
+Local Ltac derive_proj f :=
+  refine {|
+      proj := f;
+      update s m := set f (fun _ => m) s;
+  |}; crush.
+
+Definition MEM : Proj State Memory. derive_proj state_memory. Defined.
+Definition PC : Proj State Addr. derive_proj state_pc. Defined.
+Definition SP : Proj State Addr. derive_proj state_sp. Defined.
+Definition INP : Proj State (Image InputColor). derive_proj state_inp. Defined.
+Definition OUT_CHARS : Proj State (list Char). derive_proj state_chars. Defined.
+Definition OUT_BYTES : Proj State (list Byte). derive_proj state_bytes. Defined.
+Definition OUT_SOUND : Proj State Sound. derive_proj state_sound. Defined.
+Definition OUT_IMAGE : Proj State (Image (option OutputColor)). derive_proj state_image. Defined.
+Definition LOG : Proj State (list OutputFrame). derive_proj state_log. Defined.
+
+Instance independent_MEM_IMAGE: Independent MEM OUT_IMAGE. crush. Defined.
+Instance independent_MEM_BYTES: Independent MEM OUT_BYTES. crush. Defined.
+Instance independent_MEM_CHARS: Independent MEM OUT_CHARS. crush. Defined.
+Instance independent_MEM_SOUND: Independent MEM OUT_SOUND. crush. Defined.
+Instance independent_MEM_LOG:   Independent MEM LOG. crush. Defined.
+Instance independent_MEM_INP:   Independent MEM INP. crush. Defined.
+Instance independent_MEM_PC:    Independent MEM PC. crush. Defined.
+Instance independent_MEM_SP:    Independent MEM SP. crush. Defined.
+
+Instance independent_IMAGE_BYTES: Independent OUT_IMAGE OUT_BYTES. crush. Defined.
+Instance independent_IMAGE_CHARS: Independent OUT_IMAGE OUT_CHARS. crush. Defined.
+Instance independent_IMAGE_SOUND: Independent OUT_IMAGE OUT_SOUND. crush. Defined.
+Instance independent_IMAGE_LOG:   Independent OUT_IMAGE LOG. crush. Defined.
+Instance independent_IMAGE_INP:   Independent OUT_IMAGE INP. crush. Defined.
+Instance independent_IMAGE_PC:    Independent OUT_IMAGE PC. crush. Defined.
+Instance independent_IMAGE_SP:    Independent OUT_IMAGE SP. crush. Defined.
+
+Instance independent_BYTES_CHARS: Independent OUT_BYTES OUT_CHARS. crush. Defined.
+Instance independent_BYTES_SOUND: Independent OUT_BYTES OUT_SOUND. crush. Defined.
+Instance independent_BYTES_LOG:   Independent OUT_BYTES LOG. crush. Defined.
+Instance independent_BYTES_INP:   Independent OUT_BYTES INP. crush. Defined.
+Instance independent_BYTES_PC:    Independent OUT_BYTES PC. crush. Defined.
+Instance independent_BYTES_SP:    Independent OUT_BYTES SP. crush. Defined.
+
+Instance independent_CHARS_SOUND: Independent OUT_CHARS OUT_SOUND. crush. Defined.
+Instance independent_CHARS_LOG:   Independent OUT_CHARS LOG. crush. Defined.
+Instance independent_CHARS_INP:   Independent OUT_CHARS INP. crush. Defined.
+Instance independent_CHARS_PC:    Independent OUT_CHARS PC. crush. Defined.
+Instance independent_CHARS_SP:    Independent OUT_CHARS SP. crush. Defined.
+
+Instance independent_SOUND_LOG: Independent OUT_SOUND LOG. crush. Defined.
+Instance independent_SOUND_INP: Independent OUT_SOUND INP. crush. Defined.
+Instance independent_SOUND_PC:  Independent OUT_SOUND PC. crush. Defined.
+Instance independent_SOUND_SP:  Independent OUT_SOUND SP. crush. Defined.
+
+Instance independent_LOG_INP: Independent LOG INP. crush. Defined.
+Instance independent_LOG_PC:  Independent LOG PC. crush. Defined.
+Instance independent_LOG_SP:  Independent LOG SP. crush. Defined.
+
+Instance independent_INP_PC: Independent INP PC. crush. Defined.
+Instance independent_INP_SP: Independent INP SP. crush. Defined.
+
+Instance independent_PC_SP: Independent PC SP. crush. Defined.
+
+Instance concreteParams1 : @MachineParams1 concreteParams0 :=
+{
+    State := State;
+
+    MEM := MEM;
+    PC := PC;
+    SP := SP;
+
+    INP := INP;
+
+    OUT_CHARS  := OUT_CHARS ;
+    OUT_BYTES  := OUT_BYTES ;
+    OUT_SOUND  := OUT_SOUND ;
+    OUT_IMAGE  := OUT_IMAGE ;
+
+    LOG := LOG;
+
+    independent_MEM_IMAGE := independent_MEM_IMAGE;
+    independent_MEM_BYTES := independent_MEM_BYTES;
+    independent_MEM_CHARS := independent_MEM_CHARS;
+    independent_MEM_SOUND := independent_MEM_SOUND;
+    independent_MEM_LOG := independent_MEM_LOG;
+    independent_MEM_INP := independent_MEM_INP;
+    independent_MEM_PC := independent_MEM_PC;
+    independent_MEM_SP := independent_MEM_SP;
+
+    independent_IMAGE_BYTES := independent_IMAGE_BYTES;
+    independent_IMAGE_CHARS := independent_IMAGE_CHARS;
+    independent_IMAGE_SOUND := independent_IMAGE_SOUND;
+    independent_IMAGE_LOG := independent_IMAGE_LOG;
+    independent_IMAGE_INP := independent_IMAGE_INP;
+    independent_IMAGE_PC := independent_IMAGE_PC;
+    independent_IMAGE_SP := independent_IMAGE_SP;
+
+    independent_BYTES_CHARS := independent_BYTES_CHARS;
+    independent_BYTES_SOUND := independent_BYTES_SOUND;
+    independent_BYTES_LOG := independent_BYTES_LOG;
+    independent_BYTES_INP := independent_BYTES_INP;
+    independent_BYTES_PC := independent_BYTES_PC;
+    independent_BYTES_SP := independent_BYTES_SP;
+
+    independent_CHARS_SOUND := independent_CHARS_SOUND;
+    independent_CHARS_LOG := independent_CHARS_LOG;
+    independent_CHARS_INP := independent_CHARS_INP;
+    independent_CHARS_PC := independent_CHARS_PC;
+    independent_CHARS_SP := independent_CHARS_SP;
+
+    independent_SOUND_LOG := independent_SOUND_LOG;
+    independent_SOUND_INP := independent_SOUND_INP;
+    independent_SOUND_PC := independent_SOUND_PC;
+    independent_SOUND_SP := independent_SOUND_SP;
+
+    independent_LOG_INP := independent_LOG_INP;
+    independent_LOG_PC := independent_LOG_PC;
+    independent_LOG_SP := independent_LOG_SP;
+
+    independent_INP_PC := independent_INP_PC;
+    independent_INP_SP := independent_INP_SP;
+
+    independent_PC_SP := independent_PC_SP;
+}.
+
+Instance concreteParams2 : @MachineParams2 concreteParams0 concreteParams1 :=
+{
+    M := EST State;
+    H_mon := est_smonad State;
+}.
